Further progress on RC cleanup

linking/linking_inv.v
@@ -84,33 +84,24 @@ Section linkingInv.
 
 Variable N : pos.
 
-Variable cores_S' cores_T : 'I_N -> Modsem.t. 
-
+Variable cores_S cores_T : 'I_N -> Modsem.t. 
+Variable rclosed_S : forall i : 'I_N, RCSem.t (cores_S i).(sem) (cores_S i).(ge).
 Variable nucular_T : forall i : 'I_N, Nuke_sem.t (cores_T i).(sem).
 
 Variable fun_tbl : ident -> option 'I_N.
 
-Variable sims' : forall i : 'I_N, 
-  let s := cores_S' i in
+Variable sims : forall i : 'I_N, 
+  let s := cores_S i in
   let t := cores_T i in
   SM_simulation_inject s.(sem) t.(sem) s.(ge) t.(ge).
 
 Variable my_ge : ge_ty.
-Variable my_ge_S : forall (i : 'I_N), genvs_domain_eq my_ge (cores_S' i).(ge).
+Variable my_ge_S : forall (i : 'I_N), genvs_domain_eq my_ge (cores_S i).(ge).
 Variable my_ge_T : forall (i : 'I_N), genvs_domain_eq my_ge (cores_T i).(ge).
 
-Let types := fun i : 'I_N => (sims' i).(core_data).
+Let types := fun i : 'I_N => (sims i).(core_data).
 Let ords : forall i : 'I_N, types i -> types i -> Prop 
-  := fun i : 'I_N => (sims' i).(core_ord).
-
-Let cores_S (ix : 'I_N) := 
-  Modsem.mk (cores_S' ix).(ge) (RC.effsem (cores_S' ix).(sem)).
-
-Lemma sims : forall i : 'I_N,
-  let s := cores_S i in
-  let t := cores_T i in
-  SM_simulation_inject s.(sem) t.(sem) s.(ge) t.(ge).  
-Proof. by move=> ix; apply: rc_sim; apply: (sims' ix). Qed.
+  := fun i : 'I_N => (sims i).(core_ord).
 
 Let linker_S := effsem N cores_S fun_tbl.
 Let linker_T := effsem N cores_T fun_tbl.
@@ -329,8 +320,8 @@ Section vis_inv.
 
 Import Core.
 
-Record vis_inv (c : t cores_S) mu : Type :=
-  { vis_sup : {subset (RC.roots my_ge c.(Core.c)) <= vis mu} }.
+Record vis_inv (c : t cores_S) (B : block -> bool) mu : Type :=
+  { vis_sup : {subset (RC.roots my_ge (RC.mk c.(Core.c) B)) <= vis mu} }.
 
 End vis_inv.
 
@@ -358,7 +349,9 @@ Record frame_inv
   ; frame_vinj  : Forall2 (val_inject (restrict (as_inj mu0) (vis mu0))) vals1 vals2  
 
     (* source state invariants *)
-  ; frame_vis   : vis_inv c mu0
+  ; frame_vis   : exists B, 
+                  [/\ vis_inv c B mu0
+                    & RCSem.I (rclosed_S c.(i)) c.(Core.c) m10 B]
 
     (* target mu invariants *)
   ; frame_domt  : DomTgt mu0 = valid_block_dec m20
@@ -492,11 +485,13 @@ Variable  (pf : c.(i)=d.(i)).
 
 (** ** Running Cores Invariant *)
 
-Record head_inv cd (mu : Inj.t) mus m1 m2 : Type :=
+Record head_inv cd (mu : Inj.t) mus m1 m2 : Prop :=
   { head_match : (sims c.(i)).(match_state) cd mu 
                  c.(Core.c) m1 (cast'' pf d.(Core.c)) m2 
   ; head_rel   : All (rel_inv_pred m1 mu) mus 
-  ; head_vis   : vis_inv c mu 
+  ; head_vis   : exists B, 
+                 [/\ vis_inv c B mu 
+                   & RCSem.I (rclosed_S c.(i)) c.(Core.c) m1 B]
   ; head_domt  : DomTgt mu = valid_block_dec m2 
   ; head_nukeI : Nuke_sem.I (nucular_T d.(i)) d.(Core.c) m2
   ; head_gfi   : globalfunction_ptr_inject my_ge (as_inj mu)
@@ -817,7 +812,7 @@ rewrite replace_locals_locBlocksSrc in lS.
 apply/andP; split=> //.
 apply: (REACH_mono 
   (fun b0 : block =>
-    isGlobalBlock (ge (cores_S' new_ix)) b0 || getBlocks vals1 b0))=> //.
+    isGlobalBlock (ge (cores_S new_ix)) b0 || getBlocks vals1 b0))=> //.
 move=> b0; case/orP.
 by move/globs_in_frgn; apply: frgnsrc_sub_exportedsrc.
 by move=> get; apply/orP; left.
@@ -834,7 +829,7 @@ have ->: pubS' b1.
   by rewrite replace_locals_locBlocksSrc in lS.
   apply: (REACH_mono 
   (fun b0 : block =>
-    isGlobalBlock (ge (cores_S' new_ix)) b0 || getBlocks vals1 b0))=> //.
+    isGlobalBlock (ge (cores_S new_ix)) b0 || getBlocks vals1 b0))=> //.
   move=> b0; case/orP.
   by move/globs_in_frgn; apply: frgnsrc_sub_exportedsrc.
   by move=> get; apply/orP; left. }
@@ -923,7 +918,8 @@ by rewrite replace_locals_foreign.
 by rewrite /Consistent /= replace_locals_as_inj.
 case: rel=> _ _ _ H b; case/andP=> /= H2 H3; apply: H. 
 by apply/andP; split=> //=; move: H2; rewrite lo_vis.
-by case: vis=> rvis; apply: Build_vis_inv; rewrite lo_vis.
+case: vis=> B; case=> H ?; exists B; split=> //. 
+by apply: Build_vis_inv; rewrite lo_vis; case: H.
 by rewrite replace_locals_DomTgt.
 by rewrite /lo /= /lo' /= replace_locals_as_inj.
 Qed.
@@ -1164,7 +1160,8 @@ split=> /=.
 split; first by apply: (head_rel inv).
 by case: tlinv.
 split. 
-exists pf,sig_pf,cd,e,sig,args1,e,sig,args2; split=> //.
+exists pf,sig_pf,cd,e,sig,args1,e,sig,args2.
+apply: Build_frame_inv=> //.
 by apply: (head_match inv).
 by apply: (head_vis inv).
 by apply: (head_domt inv).
@@ -1444,22 +1441,20 @@ apply all_relinv_step with (s1 := STACK.pop s1) (s2 := STACK.pop s2)=> //.
 by apply: (IH all all2 _ _ frall').
 Qed.
 
-Lemma vis_inv_step (c c' : Core.t cores_S) :
-  vis_inv c mu -> 
-  RC.locs (Core.c c') 
-    = REACH m1' (fun b => structured_injections.freshloc m1 m1' b
-                       || RC.reach_set (ge (cores_S (Core.i c))) (Core.c c) m1 b) ->
+Lemma vis_inv_step (c c' : Core.t cores_S) B :
+  vis_inv c B mu -> 
   REACH_closed m1 (vis mu) -> 
-  vis_inv c' mu'.
+  vis_inv c' (REACH m1' (fun b => structured_injections.freshloc m1 m1' b
+                || RC.reach_set (ge (cores_S (Core.i c))) (RC.mk (Core.c c) B) m1 b)) mu'.
 Proof.
-move=> E C rc; move: E.
+move=> E rc; move: E.
 case=> E; apply: Build_vis_inv=> b F.
 move: F; rewrite/RC.roots/in_mem/=; move/orP=> [|F].
 move=> F.
 by apply: (intern_incr_vis _ _ incr); apply: E; apply/orP; left.
-case G: (RC.locs (Core.c c) b).
+case G: (B b).
 by apply: (intern_incr_vis _ _ incr); apply: E; apply/orP; right.
-move: C F=> -> H.
+move: F=> H.
 apply: visrc; apply: (REACH_mono _ _ _ _ _ H)=> b0 H2. 
 case: {H2}(orP H2)=> H2.
 move: alloc; rewrite sm_locally_allocatedChar /vis; case. 
@@ -1479,9 +1474,6 @@ Lemma head_inv_step
     cd cd' mus s1 s2 U n V :
   head_inv pf cd mu mus m1 m2 -> 
   frame_all mus m1 m2 s1 s2 -> 
-  RC.locs c' 
-    = REACH m1' (fun b => structured_injections.freshloc m1 m1' b
-                       || RC.reach_set (ge (cores_S (Core.i c))) (Core.c c) m1 b) ->
   effect_semantics.effstep 
     (sem (cores_S (Core.i c))) (ge (cores_S (Core.i c))) U 
     (Core.c c) m1 c' m1' -> 
@@ -1494,11 +1486,18 @@ Lemma head_inv_step
     (cast'' pf (Core.c (Core.upd d d'))) m2' -> 
   @head_inv (Core.upd c c') (Core.upd d d') pf cd' mu' mus m1' m2'.
 Proof.
-move=> hdinv frame locs effstep effstepN vgenv mtch.
+move=> hdinv frame effstep effstepN vgenv mtch.
 apply: Build_head_inv=> //.
 by apply: (all_relinv_step frame); apply: (head_rel hdinv).
-+ case: hdinv=> hdmtch ? A ? ? ?; apply: (vis_inv_step A)=> //.
-  by apply match_visible in hdmtch.
+case: hdinv=> hdmtch ?; case=> B0 []?????.
+set B := REACH m1' 
+  (fun b => structured_injections.freshloc m1 m1' b
+         || RC.reach_set (ge (cores_S (Core.i c))) 
+              (RC.mk (Core.c c) B0) m1 b).
+{ exists B; rewrite /B; move {B}; split=> //. 
+  by apply: vis_inv_step=> //; apply match_visible in hdmtch. 
+  apply RCSem.step_ax=> //.
+  by apply effax1 in effstep; case: effstep. }
 move: alloc; case/sm_locally_allocatedChar=> _ []-> []_ []H1 []_ H2.
 rewrite (head_domt hdinv); extensionality b.
 case e: (freshloc m2 m2' b). 
@@ -1545,8 +1544,7 @@ Record R (data : sig_data N (fun ix : 'I_N => (sims ix).(core_data)))
            (mu_top : Inj.t) mus, 
     [/\ mu = mu_top
       , exists pf2 : projT1 data = c.(Core.i),
-          @head_inv c d pf (cast_ty (lift_eq _ pf2) (projT2 data)) 
-          mu_top mus m1 m2 
+        @head_inv c d pf (cast_ty (lift_eq _ pf2) (projT2 data)) mu_top mus m1 m2 
       & tail_inv mus (pop s1) (pop s2) m1 m2] 
 
     (* side conditions *)
@@ -1663,19 +1661,6 @@ by case: (semantics.initial_core _ _ _ _)=> // c;
 Qed.
 
 End initCore_lems.
-
-Section initCore_lems2.
-
-Context c1 sg ix v vs (init1 : initCore cores_S sg ix v vs = Some c1).
-
-Lemma initCore_locs : RC.locs (Core.c c1) = (getBlocks vs).
-Proof.
-move: init1; rewrite /initCore /= /RC.initial_core.
-case: (initial_core _ _ _ _)=> // c. 
-by case; case: c1=> ?; case=> ? ? ? /=; case=> _ _ ->.
-Qed.
-
-End initCore_lems2.
 
 End linkingInv.
 
